Another function proof for monomorphisms

algebra_chap0.v
@@ -30,7 +30,10 @@ Section Functions.
       (f_inv b = Some a -> f a = b) /\
       (f_inv b = None -> ~exists a, f a = b).
 
-  Theorem partial_inverse_false (f: A -> B) (f_inv: partial_inverse f) :
+  Axiom partial_inverse_exists :
+    forall f, exists (f_inv : partial_inverse f), is_partial_inverse f f_inv.
+
+  Theorem partial_inverse_false f f_inv :
     is_partial_inverse f f_inv ->
     forall a, f_inv (f a) = None -> False.
   Proof.
@@ -42,10 +45,22 @@ Section Functions.
     auto.
   Qed.
 
-  Theorem left_inverse_iff_injective (f : A -> B) (f_inv: partial_inverse f) :
-    nonempty A -> is_partial_inverse f f_inv -> (exists g, left_inverse f g) <-> injective f.
+  Theorem partial_inverse_injective f f_inv :
+    injective f -> is_partial_inverse f f_inv -> forall a, f_inv (f a) = Some a.
   Proof.
-    intros [s _] PartialInverse.
+    intros f_injective PartialInverse a.
+    remember (f_inv (f a)) as Q.
+    symmetry in HeqQ.
+    destruct Q;
+      [apply PartialInverse, f_injective in HeqQ; rewrite HeqQ; reflexivity |
+       apply (partial_inverse_false _ _ PartialInverse) in HeqQ; contradict HeqQ].
+  Qed.
+
+  Theorem left_inverse_iff_injective (f : A -> B) :
+    nonempty A -> (exists g, left_inverse f g) <-> injective f.
+  Proof.
+    destruct (partial_inverse_exists f) as [f_inv PartialInverse].
+    intros [s _].
     split.
     - intros [g left_inverse] a a' H.
     apply (fun_intro _ _ g (f a) (f a')) in H.
@@ -59,27 +74,20 @@ Section Functions.
                 | None => s
                 end).
       intros a.
-      remember (f_inv (f a)) as Q.
-      symmetry in HeqQ.
-      destruct Q.
-      apply (PartialInverse (f a)) in HeqQ.
-      apply f_injective in HeqQ.
-      exact HeqQ.
-      apply (partial_inverse_false _ _ PartialInverse) in HeqQ.
-      contradict HeqQ.
+      rewrite (partial_inverse_injective _ _ f_injective PartialInverse a); auto.
   Qed.
 
-  Theorem right_inverse_iff_surjective (f : A -> B) (f_inv: partial_inverse f):
-    nonempty A -> is_partial_inverse f f_inv -> (exists g, right_inverse f g) <-> surjective f.
+  Theorem right_inverse_iff_surjective (f : A -> B):
+    nonempty A -> (exists g, right_inverse f g) <-> surjective f.
   Proof.
-    intros [s _] PartialInverse.
+    destruct (partial_inverse_exists f) as [f_inv PartialInverse].
+    intros [s _].
     split.
     - intros [g right_inverse].
       unfold surjective.
       intros b; exists (g b).
       rewrite right_inverse; reflexivity.
     - intros f_surjective.
-      unfold right_inverse.
       exists (fun b => match (f_inv b) with | Some a => a | None => s end).
       intros b.
       remember (f_inv b) as Q.
@@ -91,4 +99,21 @@ Section Functions.
       contradict HeqQ.
       apply f_surjective.
   Qed.
+
+  Definition monomorphism (f: A -> B) := forall (Z: Set) α α' (a : Z), f (α a) = f (α' a) -> α a = α' a.
+
+  Definition singleton (C: Set) := C -> Set.
+
+  Theorem monomorphism_iff_injective f :
+    nonempty A -> injective f -> monomorphism f.
+  Proof.
+    intros A_nonempty f_injective Z α α' a.
+    apply left_inverse_iff_injective in f_injective; auto.
+    destruct f_injective as [g g_left_inverse].
+    intros f_equiv.
+    apply (fun_intro _ _ g _ _) in f_equiv.
+    repeat rewrite g_left_inverse in f_equiv.
+    assumption.
+  Qed.
+
 End Functions.
